std/channel1 -> std/latch1.

theories/std/latch1.v
@@ -42,21 +42,21 @@ Implicit Types l : loc.
 Section condition.
   Context `{heap_GS : !heapGS Σ} {mutex : mutex Σ} (condition : condition mutex).
 
-  Definition channel1_create : val :=
+  Definition latch1_create : val :=
     λ: <>,
       let: "t" := record3_make #false #() #() in
       "t".[mutex] <- mutex.(mutex_create) #() ;;
       "t".[condition] <- condition.(condition_create) #() ;;
       "t".
 
-  Definition channel1_signal : val :=
+  Definition latch1_signal : val :=
     λ: "t",
       mutex.(mutex_protect) !"t".[mutex] (λ: <>,
         "t".[flag] <- #true
       ) ;;
       condition.(condition_signal) !"t".[condition].
 
-  Definition channel1_wait : val :=
+  Definition latch1_wait : val :=
     λ: "t",
       let: "mtx" := !"t".[mutex] in
       let: "cond" := !"t".[condition] in
@@ -65,98 +65,98 @@ Section condition.
       ).
 End condition.
 
-Class Channel1G Σ `{heap_GS : !heapGS Σ} := {
-  #[local] channel1_G_producer_G :: OneshotG Σ unit unit ;
-  #[local] channel1_G_consumer_G :: ExclG Σ unitO ;
+Class Latch1G Σ `{heap_GS : !heapGS Σ} := {
+  #[local] latch1_G_producer_G :: OneshotG Σ unit unit ;
+  #[local] latch1_G_consumer_G :: ExclG Σ unitO ;
 }.
 
-Definition channel1_Σ := #[
+Definition latch1_Σ := #[
   oneshot_Σ unit unit ;
   excl_Σ unitO
 ].
-#[global] Instance subG_channel1_Σ Σ `{heap_GS : !heapGS Σ} :
-  subG channel1_Σ Σ →
-  Channel1G Σ .
+#[global] Instance subG_latch1_Σ Σ `{heap_GS : !heapGS Σ} :
+  subG latch1_Σ Σ →
+  Latch1G Σ .
 Proof.
   solve_inG.
 Qed.
 
-Section channel1_G.
-  Context `{channel1_G : Channel1G Σ}.
+Section latch1_G.
+  Context `{latch1_G : Latch1G Σ}.
   Context {mutex : mutex Σ} (condition : condition mutex).
 
-  Record channel1_meta := {
-    channel1_meta_producer : gname ;
-    channel1_meta_consumer : gname ;
+  Record latch1_meta := {
+    latch1_meta_producer : gname ;
+    latch1_meta_consumer : gname ;
   }.
-  Implicit Types γ : channel1_meta.
+  Implicit Types γ : latch1_meta.
 
-  #[local] Instance channel1_meta_eq_dec : EqDecision channel1_meta :=
+  #[local] Instance latch1_meta_eq_dec : EqDecision latch1_meta :=
     ltac:(solve_decision).
-  #[local] Instance channel1_meta_countable :
-    Countable channel1_meta.
+  #[local] Instance latch1_meta_countable :
+    Countable latch1_meta.
   Proof.
     pose encode γ := (
-      γ.(channel1_meta_producer),
-      γ.(channel1_meta_consumer)
+      γ.(latch1_meta_producer),
+      γ.(latch1_meta_consumer)
     ).
     pose decode := λ '(γ_producer, γ_consumer), {|
-      channel1_meta_producer := γ_producer ;
-      channel1_meta_consumer := γ_consumer ;
+      latch1_meta_producer := γ_producer ;
+      latch1_meta_consumer := γ_consumer ;
     |}.
     refine (inj_countable' encode decode _). intros []. done.
   Qed.
 
-  #[local] Definition channel1_inv_inner l γ P : iProp Σ :=
+  #[local] Definition latch1_inv_inner l γ P : iProp Σ :=
     ∃ b,
     l.[flag] ↦ #b ∗
     if b then
-      oneshot_shot γ.(channel1_meta_producer) () ∗
+      oneshot_shot γ.(latch1_meta_producer) () ∗
       ( P
-      ∨ excl γ.(channel1_meta_consumer) ()
+      ∨ excl γ.(latch1_meta_consumer) ()
       )
     else
-      oneshot_pending γ.(channel1_meta_producer) (DfracOwn (1/3)) ().
-  #[local] Definition channel1_inv t P : iProp Σ :=
+      oneshot_pending γ.(latch1_meta_producer) (DfracOwn (1/3)) ().
+  #[local] Definition latch1_inv t P : iProp Σ :=
     ∃ l γ mtx cond,
     ⌜t = #l⌝ ∗
     meta l nroot γ ∗
     l.[mutex] ↦□ mtx ∗
-    mutex.(mutex_inv) mtx (channel1_inv_inner l γ P) ∗
+    mutex.(mutex_inv) mtx (latch1_inv_inner l γ P) ∗
     l.[condition] ↦□ cond ∗
     condition.(condition_inv) cond.
 
-  Definition channel1_producer t : iProp Σ :=
+  Definition latch1_producer t : iProp Σ :=
     ∃ l γ,
     ⌜t = #l⌝ ∗
     meta l nroot γ ∗
-    oneshot_pending γ.(channel1_meta_producer) (DfracOwn (2/3)) ().
+    oneshot_pending γ.(latch1_meta_producer) (DfracOwn (2/3)) ().
 
-  Definition channel1_consumer t : iProp Σ :=
+  Definition latch1_consumer t : iProp Σ :=
     ∃ l γ,
     ⌜t = #l⌝ ∗
     meta l nroot γ ∗
-    excl γ.(channel1_meta_consumer) ().
+    excl γ.(latch1_meta_consumer) ().
 
-  #[global] Instance channel1_inv_persistent t P :
-    Persistent (channel1_inv t P).
+  #[global] Instance latch1_inv_persistent t P :
+    Persistent (latch1_inv t P).
   Proof.
     apply _.
   Qed.
-  #[global] Instance channel1_producer_timeless t :
-    Timeless (channel1_producer t).
+  #[global] Instance latch1_producer_timeless t :
+    Timeless (latch1_producer t).
   Proof.
     apply _.
   Qed.
-  #[global] Instance channel1_consumer_timeless t :
-    Timeless (channel1_consumer t).
+  #[global] Instance latch1_consumer_timeless t :
+    Timeless (latch1_consumer t).
   Proof.
     apply _.
   Qed.
 
-  Lemma channel1_producer_exclusive t :
-    channel1_producer t -∗
-    channel1_producer t -∗
+  Lemma latch1_producer_exclusive t :
+    latch1_producer t -∗
+    latch1_producer t -∗
     False.
   Proof.
     iIntros "(%l & %γ & -> & #Hmeta & Hpending) (%_l & %_γ & %Heq & _Hmeta & Hpending')". injection Heq as <-.
@@ -164,9 +164,9 @@ Section channel1_G.
     iDestruct (oneshot_pending_valid_2 with "Hpending Hpending'") as %(? & _). done.
   Qed.
 
-  Lemma channel1_consumer_exclusive t :
-    channel1_consumer t -∗
-    channel1_consumer t -∗
+  Lemma latch1_consumer_exclusive t :
+    latch1_consumer t -∗
+    latch1_consumer t -∗
     False.
   Proof.
     iIntros "(%l & %γ & -> & #Hmeta & Hexcl) (%_l & %_γ & %Heq & _Hmeta & Hexcl')". injection Heq as <-.
@@ -174,14 +174,14 @@ Section channel1_G.
     iDestruct (excl_exclusive with "Hexcl Hexcl'") as %[].
   Qed.
 
-  Lemma channel1_create_spec P :
+  Lemma latch1_create_spec P :
     {{{ True }}}
-      channel1_create condition #()
+      latch1_create condition #()
     {{{ t,
       RET t;
-      channel1_inv t P ∗
-      channel1_producer t ∗
-      channel1_consumer t
+      latch1_inv t P ∗
+      latch1_producer t ∗
+      latch1_consumer t
     }}}.
   Proof.
     iIntros "%Φ _ HΦ".
@@ -195,15 +195,15 @@ Section channel1_G.
     iEval (assert (1 = 2/3 + 1/3)%Qp as -> by compute_done) in "Hpending".
     iDestruct "Hpending" as "(Hpending1 & Hpending2)".
 
-    iMod (excl_alloc (excl_G := channel1_G_consumer_G) ()) as "(%γ_consumer & Hexcl)".
+    iMod (excl_alloc (excl_G := latch1_G_consumer_G) ()) as "(%γ_consumer & Hexcl)".
 
     pose γ := {|
-      channel1_meta_producer := γ_producer ;
-      channel1_meta_consumer := γ_consumer ;
+      latch1_meta_producer := γ_producer ;
+      latch1_meta_consumer := γ_consumer ;
     |}.
     iMod (meta_set _ _ γ nroot with "Hmeta") as "#Hmeta"; first done.
 
-    wp_smart_apply (mutex_create_spec _ (channel1_inv_inner l γ P) with "[Hflag Hpending2]") as "%mtx #Hmtx_inv"; first iSteps.
+    wp_smart_apply (mutex_create_spec _ (latch1_inv_inner l γ P) with "[Hflag Hpending2]") as "%mtx #Hmtx_inv"; first iSteps.
     wp_store.
     iMod (mapsto_persist with "Hmtx") as "Hmtx".
 
@@ -214,13 +214,13 @@ Section channel1_G.
     iSteps.
   Qed.
 
-  Lemma channel1_signal_spec t P :
+  Lemma latch1_signal_spec t P :
     {{{
-      channel1_inv t P ∗
-      channel1_producer t ∗
+      latch1_inv t P ∗
+      latch1_producer t ∗
       P
     }}}
-      channel1_signal condition t
+      latch1_signal condition t
     {{{
       RET #(); True
     }}}.
@@ -243,12 +243,12 @@ Section channel1_G.
     iSteps.
   Qed.
 
-  Lemma channel1_wait_spec t P :
+  Lemma latch1_wait_spec t P :
     {{{
-      channel1_inv t P ∗
-      channel1_consumer t
+      latch1_inv t P ∗
+      latch1_consumer t
     }}}
-      channel1_wait condition t
+      latch1_wait condition t
     {{{
       RET #();
       P
@@ -264,7 +264,7 @@ Section channel1_G.
         if b then
           P
         else
-          excl γ.(channel1_meta_consumer) ()
+          excl γ.(latch1_meta_consumer) ()
       )%I).
       wp_smart_apply (condition_wait_until_spec _ Ψ with "[$Hcond_inv $Hmtx_inv $Hmtx_locked $Hsignal_inv $Hexcl]").
       { clear. iStep 15 as (Φ b) "Hb Hexcl Hflag".
@@ -276,12 +276,12 @@ Section channel1_G.
     }
     iSteps.
   Qed.
-End channel1_G.
+End latch1_G.
 
-#[global] Opaque channel1_create.
-#[global] Opaque channel1_wait.
-#[global] Opaque channel1_signal.
+#[global] Opaque latch1_create.
+#[global] Opaque latch1_wait.
+#[global] Opaque latch1_signal.
 
-#[global] Opaque channel1_inv.
-#[global] Opaque channel1_producer.
-#[global] Opaque channel1_consumer.
+#[global] Opaque latch1_inv.
+#[global] Opaque latch1_producer.
+#[global] Opaque latch1_consumer.
